Add a data invariant to the monotonic heap model

ulib/FStar.Monotonic.Heap.fsti
@@ -4,11 +4,12 @@ module S  = FStar.Set
 module TS = FStar.TSet
 
 open FStar.Preorder
+open FStar.DataInvariant
 
 let set  = Set.set
 let tset = TSet.set
 
-val heap :Type u#1
+val heap : Type u#1
 
 val equal: heap -> heap -> Type0
 
@@ -18,82 +19,82 @@ val equal_extensional (h1:heap) (h2:heap)
 
 val emp :heap
 
-val mref (a:Type0) (rel:preorder a) :Type0
+val mref (a:Type0) (inv:data_inv a) (rel:preorder a):Type0
 
-val addr_of: #a:Type0 -> #rel:preorder a -> mref a rel -> GTot nat
+val addr_of: #a:Type0 -> #inv:data_inv a -> #rel:preorder a -> mref a inv rel -> GTot nat
 
-val is_mm: #a:Type0 -> #rel:preorder a -> mref a rel -> GTot bool
+val is_mm: #a:Type0 -> #inv:data_inv a -> #rel:preorder a -> mref a inv rel -> GTot bool
 
 val compare_addrs:
-  #a:Type0 -> #b:Type0 -> #rel1:preorder a -> #rel2:preorder b ->
-  r1:mref a rel1 -> r2:mref b rel2 -> Tot (b:bool{b = (addr_of r1 = addr_of r2)})
+  #a:Type0 -> #b:Type0 -> (#inv1:data_inv a) -> (#inv2:data_inv b) -> #rel1:preorder a -> #rel2:preorder b ->
+  r1:mref a inv1 rel1 -> r2:mref b inv2 rel2 -> Tot (b:bool{b = (addr_of r1 = addr_of r2)})
 
-val contains: #a:Type0 -> #rel:preorder a -> heap -> mref a rel -> Type0
+val contains: #a:Type0 -> #inv:data_inv a -> #rel:preorder a -> heap -> mref a inv rel -> Type0
 
 val addr_unused_in: nat -> heap -> Type0
 
-val unused_in: #a:Type0 -> #rel:preorder a -> mref a rel -> heap -> Type0
+val unused_in: #a:Type0 -> #inv:data_inv a -> #rel:preorder a -> mref a inv rel -> heap -> Type0
 
-let fresh (#a:Type) (#rel:preorder a) (r:mref a rel) (h0:heap) (h1:heap) =
+let fresh (#a:Type) (#inv:data_inv a) (#rel:preorder a) (r:mref a inv rel) (h0:heap) (h1:heap) =
   r `unused_in` h0 /\ h1 `contains` r
 
-let only_t (#a:Type0) (#rel:preorder a) (x:mref a rel) :GTot (tset nat) = TS.singleton (addr_of x)
+let only_t (#a:Type0) (#inv:data_inv a) (#rel:preorder a) (x:mref a inv rel) :GTot (tset nat) = TS.singleton (addr_of x)
 
-let only (#a:Type0) (#rel:preorder a) (x:mref a rel) :GTot (set nat) = S.singleton (addr_of x)
+let only (#a:Type0) (#inv:data_inv a) (#rel:preorder a) (x:mref a inv rel) :GTot (set nat) = S.singleton (addr_of x)
 
-let op_Hat_Plus_Plus (#a:Type0) (#rel:preorder a) (r:mref a rel) (s:set nat) :GTot (set nat) = S.union (only r) s
+let op_Hat_Plus_Plus (#a:Type0) (#inv:data_inv a) (#rel:preorder a) (r:mref a inv rel) (s:set nat) :GTot (set nat) = S.union (only r) s
 
-let op_Plus_Plus_Hat (#a:Type0) (#rel:preorder a) (s:set nat) (r:mref a rel) :GTot (set nat) = S.union s (only r)
+let op_Plus_Plus_Hat (#a:Type0) (#inv:data_inv a) (#rel:preorder a) (s:set nat) (r:mref a inv rel) :GTot (set nat) = S.union s (only r)
 
-let op_Hat_Plus_Hat (#a:Type0) (#b:Type0) (#rel1:preorder a) (#rel2:preorder b) (r1:mref a rel1) (r2:mref b rel2)
+let op_Hat_Plus_Hat (#a:Type0) (#b:Type0) (#inv1:data_inv a) (#inv2:data_inv b) (#rel1:preorder a) (#rel2:preorder b) (r1:mref a inv1 rel1) (r2:mref b inv2 rel2)
   :GTot (set nat) = S.union (only r1) (only r2)
 
-val sel_tot: #a:Type0 -> #rel:preorder a -> h:heap -> r:mref a rel{h `contains` r} -> Tot a
+val sel_tot: #a:Type0 -> #inv:data_inv a -> #rel:preorder a -> h:heap -> r:mref a inv rel{h `contains` r} -> Tot a
 
-val sel: #a:Type0 -> #rel:preorder a -> heap -> mref a rel -> GTot a
+val sel: #a:Type0 -> #inv:data_inv a -> #rel:preorder a -> heap -> mref a inv rel -> GTot a
 
-let valid_upd (#a:Type0) (#rel:preorder a) (h:heap) (r:mref a rel) (x:a) = rel (sel h r) x
+let valid_upd (#a:Type0) (#inv:data_inv a) (#rel:preorder a) (h:heap) (r:mref a inv rel) (x:a) = rel (sel h r) x
 
-val upd_tot: #a:Type0 -> #rel:preorder a -> h:heap -> r:mref a rel{h `contains` r} -> x:a{valid_upd h r x} -> Tot heap
+val upd_tot: #a:Type0 -> #inv:data_inv a -> #rel:preorder a -> h:heap -> r:mref a inv rel{h `contains` r} -> x:a{valid_upd h r x} -> Tot heap
 
-val upd: #a:Type0 -> #rel:preorder a -> h:heap -> r:mref a rel -> x:a{valid_upd h r x} -> GTot heap
+val upd: #a:Type0 -> #inv:data_inv a -> #rel:preorder a -> h:heap -> r:mref a inv rel -> x:a{valid_upd h r x} -> GTot heap
 
-val alloc: #a:Type0 -> rel:preorder a -> heap -> a -> mm:bool -> Tot (mref a rel * heap)
+val alloc: #a:Type0 -> inv:data_inv a -> rel:preorder a -> heap -> a -> mm:bool -> Tot (mref a inv rel * heap)
 
-val free_mm: #a:Type0 -> #rel:preorder a -> h:heap -> r:mref a rel{h `contains` r /\ is_mm r} -> GTot heap
+val free_mm: #a:Type0 -> #inv:data_inv a -> #rel:preorder a -> h:heap -> r:mref a inv rel{h `contains` r /\ is_mm r} -> GTot heap
 
 let modifies_t (s:tset nat) (h0:heap) (h1:heap) =
-  (forall (a:Type) (rel:preorder a) (r:mref a rel).{:pattern (sel h1 r)}
+  (forall (a:Type) (inv:data_inv a) (rel:preorder a) (r:mref a inv rel).{:pattern (sel h1 r)}
                                ((~ (TS.mem (addr_of r) s)) /\ h0 `contains` r) ==> sel h1 r == sel h0 r) /\
-  (forall (a:Type) (rel:preorder a) (r:mref a rel).{:pattern (contains h1 r)}
+  (forall (a:Type) (inv:data_inv a) (rel:preorder a) (r:mref a inv rel).{:pattern (contains h1 r)}
                                h0 `contains` r ==> h1 `contains` r) /\
-  (forall (a:Type) (rel:preorder a) (r:mref a rel).{:pattern (r `unused_in` h0)}
+  (forall (a:Type) (inv:data_inv a) (rel:preorder a) (r:mref a inv rel).{:pattern (r `unused_in` h0)}
                                r `unused_in` h1 ==> r `unused_in` h0)
 
 let modifies (s:set nat) (h0:heap) (h1:heap) = modifies_t (TS.tset_of_set s) h0 h1
 
 let equal_dom (h1:heap) (h2:heap) :GTot Type0 =
-  (forall (a:Type0) (rel:preorder a) (r:mref a rel). h1 `contains` r <==> h2 `contains` r) /\
-  (forall (a:Type0) (rel:preorder a) (r:mref a rel). r `unused_in` h1 <==> r `unused_in` h2)
+  (forall (a:Type0) (inv:data_inv a)(rel:preorder a) (r:mref a inv rel). h1 `contains` r <==> h2 `contains` r) /\
+  (forall (a:Type0) (inv:data_inv a)(rel:preorder a) (r:mref a inv rel). r `unused_in` h1 <==> r `unused_in` h2)
 
-val lemma_ref_unused_iff_addr_unused (#a:Type0) (#rel:preorder a) (h:heap) (r:mref a rel)
+val lemma_ref_unused_iff_addr_unused (#a:Type0) (#inv:data_inv a)(#rel:preorder a) (h:heap) (r:mref a inv rel)
   :Lemma (requires True)
          (ensures  (r `unused_in` h <==> addr_of r `addr_unused_in` h))
 	 [SMTPatOr [[SMTPat (r `unused_in` h)]; [SMTPat (addr_of r `addr_unused_in` h)]]]
 
-val lemma_contains_implies_used (#a:Type0) (#rel:preorder a) (h:heap) (r:mref a rel)
+val lemma_contains_implies_used (#a:Type0) (#inv:data_inv a)(#rel:preorder a) (h:heap) (r:mref a inv rel)
   :Lemma (requires (h `contains` r))
          (ensures  (~ (r `unused_in` h)))
 	 [SMTPatOr [[SMTPat (h `contains` r)]; [SMTPat (r `unused_in` h)]]]
 
 val lemma_distinct_addrs_distinct_types
-  (#a:Type0) (#b:Type0) (#rel1:preorder a) (#rel2:preorder b) (h:heap) (r1:mref a rel1) (r2:mref b rel2)
+  (#a:Type0) (#b:Type0) (#inv1:data_inv a) (#inv2:data_inv b) (#rel1:preorder a) (#rel2:preorder b) (h:heap) (r1:mref a inv1 rel1) (r2:mref b inv2 rel2)
   :Lemma (requires (a =!= b /\ h `contains` r1 /\ h `contains` r2))
          (ensures  (addr_of r1 <> addr_of r2))
 	 [SMTPatT (h `contains` r1); SMTPatT (h `contains` r2)]
 
 val lemma_distinct_addrs_distinct_preorders
-  (#a:Type0) (#rel1:preorder a) (#rel2:preorder a) (h:heap) (r1:mref a rel1) (r2:mref a rel2)
+  (#a:Type0) (#inv1 #inv2:data_inv a) (#rel1:preorder a) (#rel2:preorder a) (h:heap) (r1:mref a inv1 rel1) (r2:mref a inv2 rel2)
   :Lemma (requires (rel1 =!= rel2 /\ h `contains` r1 /\ h `contains` r2))
          (ensures  (addr_of r1 <> addr_of r2))
 	 [SMTPatT (h `contains` r1); SMTPatT (h `contains` r2)]
@@ -104,35 +105,35 @@ val lemma_distinct_addrs_distinct_preorders
  * automatically? should dig into smt encoding to figure.
  *)
 val lemma_distinct_addrs_unused
-  (#a:Type0) (#b:Type0) (#rel1:preorder a) (#rel2:preorder b) (h:heap) (r1:mref a rel1) (r2:mref b rel2)
+  (#a:Type0) (#b:Type0) (#inv1:data_inv a) (#inv2:data_inv b)(#rel1:preorder a) (#rel2:preorder b) (h:heap) (r1:mref a inv1 rel1) (r2:mref b inv2 rel2)
   :Lemma (requires (r1 `unused_in` h /\ ~ (r2 `unused_in` h)))
          (ensures  (addr_of r1 <> addr_of r2 /\ (~ (r1 === r2))))
          [SMTPat (r1 `unused_in` h); SMTPat (r2 `unused_in` h)]
 
-val lemma_alloc (#a:Type0) (rel:preorder a) (h0:heap) (x:a) (mm:bool)
+val lemma_alloc (#a:Type0) (inv:data_inv a) (rel:preorder a) (h0:heap) (x:a) (mm:bool)
   :Lemma (requires True)
-         (ensures  (let r, h1 = alloc rel h0 x mm in
+         (ensures  (let r, h1 = alloc inv rel h0 x mm in
                     fresh r h0 h1 /\ valid_upd h0 r x /\ h1 == upd h0 r x /\ is_mm r = mm))
-	 [SMTPat (alloc rel h0 x mm)]
+	 [SMTPat (alloc inv rel h0 x mm)]
 
 val lemma_free_mm_sel
-  (#a:Type0) (#b:Type0) (#rel1:preorder a) (#rel2:preorder b) (h0:heap)
-  (r1:mref a rel1{h0 `contains` r1 /\ is_mm r1}) (r2:mref b rel2)
+  (#a:Type0) (#b:Type0) (#inv1:data_inv a) (#inv2:data_inv b) (#rel1:preorder a) (#rel2:preorder b) (h0:heap)
+  (r1:mref a inv1 rel1{h0 `contains` r1 /\ is_mm r1}) (r2:mref b inv2 rel2)
   :Lemma (requires True)
          (ensures  (addr_of r2 <> addr_of r1 ==> sel h0 r2 == sel (free_mm h0 r1) r2))
 	 [SMTPat (sel (free_mm h0 r1) r2)]
 
 val lemma_free_mm_contains
-  (#a:Type0) (#b:Type0) (#rel1:preorder a) (#rel2:preorder b) (h0:heap)
-  (r1:mref a rel1{h0 `contains` r1 /\ is_mm r1}) (r2:mref b rel2)
+  (#a:Type0) (#b:Type0) (#inv1:data_inv a) (#inv2:data_inv b) (#rel1:preorder a) (#rel2:preorder b) (h0:heap)
+  (r1:mref a inv1 rel1{h0 `contains` r1 /\ is_mm r1}) (r2:mref b inv2 rel2)
   :Lemma (requires True)
          (ensures  (let h1 = free_mm h0 r1 in
 	            (addr_of r2 <> addr_of r1 /\ h0 `contains` r2) <==> h1 `contains` r2))
 	 [SMTPat ((free_mm h0 r1) `contains` r2)]
 
 val lemma_free_mm_unused
-  (#a:Type0) (#b:Type0) (#rel1:preorder a) (#rel2:preorder b) (h0:heap)
-  (r1:mref a rel1{h0 `contains` r1 /\ is_mm r1}) (r2:mref b rel2)
+  (#a:Type0) (#b:Type0) (#inv1:data_inv a) (#inv2:data_inv b) (#rel1:preorder a) (#rel2:preorder b) (h0:heap)
+  (r1:mref a inv1 rel1{h0 `contains` r1 /\ is_mm r1}) (r2:mref b inv2 rel2)
   :Lemma (requires True)
          (ensures  (let h1 = free_mm h0 r1 in
 	            ((addr_of r1 = addr_of r2 ==> r2 `unused_in` h1)      /\
@@ -143,7 +144,7 @@ val lemma_free_mm_unused
 (*
  * AR: we can prove this lemma only if both the mreferences have same preorder
  *)
-val lemma_sel_same_addr (#a:Type0) (#rel:preorder a) (h:heap) (r1:mref a rel) (r2:mref a rel)
+val lemma_sel_same_addr (#a:Type0) (#inv:data_inv a) (#rel:preorder a) (h:heap) (r1:mref a inv rel) (r2:mref a inv rel)
   :Lemma (requires (h `contains` r1 /\ addr_of r1 = addr_of r2))
          (ensures  (h `contains` r2 /\ sel h r1 == sel h r2))
 	 [SMTPat (sel h r1); SMTPat (sel h r2)]
@@ -151,38 +152,40 @@ val lemma_sel_same_addr (#a:Type0) (#rel:preorder a) (h:heap) (r1:mref a rel) (r
 (*
  * AR: this is true only if the preorder is same, else r2 may not be contained in h
  *)
-val lemma_sel_upd1 (#a:Type0) (#rel:preorder a) (h:heap) (r1:mref a rel) (x:a{valid_upd h r1 x}) (r2:mref a rel)
+val lemma_sel_upd1 (#a:Type0) (#inv:data_inv a) (#rel:preorder a) (h:heap) (r1:mref a inv rel) (x:a{valid_upd h r1 x}) (r2:mref a inv rel)
   :Lemma (requires (addr_of r1 = addr_of r2))
          (ensures  (sel (upd h r1 x) r2 == x))
          [SMTPat (sel (upd h r1 x) r2)]
 
-val lemma_sel_upd2 (#a:Type0) (#b:Type0) (#rel1:preorder a) (#rel2:preorder b) (h:heap) (r1:mref a rel1) (r2:mref b rel2) (x:b{valid_upd h r2 x})
+val lemma_sel_upd2 (#a:Type0) (#b:Type0) (#inv1:data_inv a) (#inv2:data_inv b)
+  (#rel1:preorder a) (#rel2:preorder b) (h:heap) (r1:mref a inv1 rel1) (r2:mref b inv2 rel2) (x:b{valid_upd h r2 x})
   :Lemma (requires (addr_of r1 <> addr_of r2))
          (ensures  (sel (upd h r2 x) r1 == sel h r1))
 	 [SMTPat (sel (upd h r2 x) r1)]
 
 val lemma_mref_injectivity
-  :(u:unit{forall (a:Type0) (b:Type0) (rel1:preorder a) (rel2:preorder b) (r1:mref a rel1) (r2:mref b rel2). a =!= b ==> ~ (eq3 r1 r2)})
+  :(u:unit{forall (a:Type0) (b:Type0) (#inv1:data_inv a) (#inv2:data_inv b) (rel1:preorder a) (rel2:preorder b) (r1:mref a inv1 rel1) (r2:mref b inv2 rel2). a =!= b ==> ~ (eq3 r1 r2)})
 
-val lemma_in_dom_emp (#a:Type0) (#rel:preorder a) (r:mref a rel)
+val lemma_in_dom_emp (#a:Type0) (#inv:data_inv a) (#rel:preorder a) (r:mref a inv rel)
   :Lemma (requires True)
          (ensures  (r `unused_in` emp))
 	 [SMTPat (r `unused_in` emp)]
 
-val lemma_upd_contains (#a:Type0) (#rel:preorder a) (h:heap) (r:mref a rel) (x:a{valid_upd h r x})
+val lemma_upd_contains (#a:Type0) (#inv:data_inv a) (#rel:preorder a) (h:heap) (r:mref a inv rel) (x:a{valid_upd h r x})
   :Lemma (requires True)
          (ensures  ((upd h r x) `contains` r))
 	 [SMTPat ((upd h r x) `contains` r)]
 
 val lemma_well_typed_upd_contains
-  (#a:Type0) (#b:Type0) (#rel1:preorder a) (#rel2:preorder b) (h:heap) (r1:mref a rel1) (x:a{valid_upd h r1 x}) (r2:mref b rel2)
+  (#a:Type0) (#b:Type0) (#inv1:data_inv a) (#inv2:data_inv b) (#rel1:preorder a) (#rel2:preorder b) (h:heap) (r1:mref a inv1 rel1) (x:a{valid_upd h r1 x}) (r2:mref b inv2 rel2)
   :Lemma (requires (h `contains` r1))
          (ensures  (let h1 = upd h r1 x in
 	            h1 `contains` r2 <==> h `contains` r2))
 	 [SMTPat ((upd h r1 x) `contains` r2)]
 
 val lemma_unused_upd_contains
-  (#a:Type0) (#b:Type0) (#rel1:preorder a) (#rel2:preorder b) (h:heap) (r1:mref a rel1) (x:a{valid_upd h r1 x}) (r2:mref b rel2)
+  (#a:Type0) (#b:Type0) (#inv1:data_inv a) (#inv2:data_inv b) (#rel1:preorder a) (#rel2:preorder b) (h:heap)
+  (r1:mref a inv1 rel1) (x:a{valid_upd h r1 x}) (r2:mref b inv2 rel2)
   :Lemma (requires (r1 `unused_in` h))
          (ensures  (let h1 = upd h r1 x in
 	            (h `contains` r2  ==> h1 `contains` r2) /\
@@ -190,42 +193,42 @@ val lemma_unused_upd_contains
 	 [SMTPat ((upd h r1 x) `contains` r2)]
 
 val lemma_upd_contains_different_addr
-  (#a:Type0) (#b:Type0) (#rel1:preorder a) (#rel2:preorder b) (h:heap) (r1:mref a rel1) (x:a{valid_upd h r1 x}) (r2:mref b rel2)
+  (#a:Type0) (#b:Type0) (#inv1:data_inv a) (#inv2:data_inv b) (#rel1:preorder a) (#rel2:preorder b) (h:heap) (r1:mref a inv1 rel1) (x:a{valid_upd h r1 x}) (r2:mref b inv2 rel2)
   :Lemma (requires (h `contains` r2 /\ addr_of r1 <> addr_of r2))
          (ensures  ((upd h r1 x) `contains` r2))
 	 [SMTPat ((upd h r1 x) `contains` r2)]
 
 val lemma_upd_unused
-  (#a:Type0) (#b:Type0) (#rel1:preorder a) (#rel2:preorder b) (h:heap) (r1:mref a rel1) (x:a{valid_upd h r1 x}) (r2:mref b rel2)
+  (#a:Type0) (#b:Type0) (#inv1:data_inv a) (#inv2:data_inv b) (#rel1:preorder a) (#rel2:preorder b) (h:heap) (r1:mref a inv1 rel1) (x:a{valid_upd h r1 x}) (r2:mref b inv2 rel2)
   :Lemma (requires True)
          (ensures  ((addr_of r1 <> addr_of r2 /\ r2 `unused_in` h) <==> r2 `unused_in` (upd h r1 x)))
 	 [SMTPat (r2 `unused_in` (upd h r1 x))]
 
-val lemma_contains_upd_modifies (#a:Type0) (#rel:preorder a) (h:heap) (r:mref a rel) (x:a{valid_upd h r x})
+val lemma_contains_upd_modifies (#a:Type0) (#inv:data_inv a) (#rel:preorder a) (h:heap) (r:mref a inv rel) (x:a{valid_upd h r x})
   :Lemma (requires (h `contains` r))
          (ensures  (modifies (S.singleton (addr_of r)) h (upd h r x)))
          [SMTPat (upd h r x); SMTPatT (h `contains` r)]
 
-val lemma_unused_upd_modifies (#a:Type0) (#rel:preorder a) (h:heap) (r:mref a rel) (x:a{valid_upd h r x})
+val lemma_unused_upd_modifies (#a:Type0) (#inv:data_inv a) (#rel:preorder a) (h:heap) (r:mref a inv rel) (x:a{valid_upd h r x})
   :Lemma (requires (r `unused_in` h))
          (ensures  (modifies (Set.singleton (addr_of r)) h (upd h r x)))
          [SMTPat (upd h r x); SMTPatT (r `unused_in` h)]
 
 val upd_upd_same_mref
-  (#a:Type) (#rel:preorder a) (h:heap) (r:mref a rel)
+  (#a:Type) (#inv:data_inv a) (#rel:preorder a) (h:heap) (r:mref a inv rel)
   (x:a{valid_upd h r x}) (y:a{valid_upd (upd h r x) r y})
   :Lemma (requires True)
          (ensures  (valid_upd h r y /\ (upd (upd h r x) r y == upd h r y)))
 	 [SMTPat (upd (upd h r x) r y)]
 
 val lemma_sel_equals_sel_tot_for_contained_refs
-  (#a:Type0) (#rel:preorder a) (h:heap) (r:mref a rel{h `contains` r})
+  (#a:Type0) (#inv:data_inv a) (#rel:preorder a) (h:heap) (r:mref a inv rel{h `contains` r})
   :Lemma (requires True)
          (ensures  (sel_tot h r == sel h r))
 	 [SMTPat (sel_tot h r)]
 
 val lemma_upd_equals_upd_tot_for_contained_refs
-  (#a:Type0) (#rel:preorder a) (h:heap) (r:mref a rel{h `contains` r}) (x:a{valid_upd h r x})
+  (#a:Type0) (#inv:data_inv a) (#rel:preorder a) (h:heap) (r:mref a inv rel{h `contains` r}) (x:a{valid_upd h r x})
   :Lemma (requires True)
          (ensures  (upd_tot h r x == upd h r x))
 	 [SMTPat (upd_tot h r x)]
