ulib/FStar.DataInvariant.fst
@@ -1,0 +1,3 @@
+module FStar.DataInvariant
+
+type data_inv (a : Type0) = a -> Type0
